### **Generic Steps to Differentiate an Inverse Function at a Point**  

These steps work for any invertible, differentiable function. Let’s break it down:

---

### **Step 1: Verify Invertibility**  
Ensure $f$ is **one-to-one** (strictly monotonic or passes the horizontal line test).  
*(If not, restrict the domain.)*

---

### **Step 2: Identify the Point**  
Find the $x$-value in the **original function** that corresponds to the $y$-value where you want the inverse’s derivative:  

$`\text{Solve } y = f(a) \text{ for } a.`$

- **Example:** If finding $(f^{-1})'(5)$, solve $f(a) = 5$.

---

### **Step 3: Compute $f'(x)$**  
Differentiate $`f(x)`$ to find $`f'(x)`$, then evaluate at $`x = a`$:  

$`f'(a) = \left. \frac{d}{dx}f(x) \right|_{x=a}.`$

- **Example:** If $f(x) = x^3$, then $f'(x) = 3x^2$, so $f'(2) = 12$.

---

### **Step 4: Apply the Inverse Derivative Formula**  
Use the key formula:  

$`(f^{-1})'(y) = \frac{1}{f'(a)} \quad \text{where} \quad y = f(a).`$
  
- **Translation:** The slope of $`f^{-1}`$ at $y$ is the reciprocal of $f$’s slope at $x = a$.

---

### **Step 5: Simplify (if Needed)**  
Rewrite the result in terms of $y$ if required.  
- **Example:** If $`f(x) = e^x`$, then $`(f^{-1})'(1) = 1`$ (since $`f^{-1}(y) = \ln y`$ and $f'(0) = 1$).

---

### **Why It Works (Intuition)**  
- The inverse function "flips" $x$ and $y$, so its slope is the reciprocal of the original slope at the mirrored point.  
- Graphically: If $f$ is steep at $`(a, y)`$, $`f^{-1}`$ is shallow at $(y, a)$, and vice versa.

---

### **Example Walkthrough**  
**Problem:** Let $`f(x) = \sqrt{x}`$. Find $`(f^{-1})'(2)`$.  

1. **Invertibility:** $f(x)$ is one-to-one for $x \geq 0$.  
2. **Find $a$:** Solve $`2 = \sqrt{a} \implies a = 4`$.  
3. **Compute $`f'(x)`$:** $`f'(x) = \frac{1}{2\sqrt{x}}`$, so $`f'(4) = \frac{1}{4}`$.  
4. **Apply formula:** $`(f^{-1})'(2) = \frac{1}{f'(4)} = 4`$.  

*(Note: Here, $`f^{-1}(y) = y^2`$, and indeed $`\frac{d}{dy} y^2 = 2y`$, which equals $4$ at $y = 2$.)*  

---

### **Key Pitfalls to Avoid**  
1. **Invertibility:** Ensure $f$ is one-to-one on the domain.  
2. **Chain Rule:** If $f$ is defined implicitly, use implicit differentiation.  
3. **Notation:** Remember $`(f^{-1})'(y)`$ is evaluated at $y-values$, not $x-values$.  

---

### **Final Answer Template**  
For any $y = f(a)$:  

$`(f^{-1})'(y) = \frac{1}{f'(a)} \quad \text{where} \quad f(a) = y.`$
  

**Shortcut for Nerds:** If $f^{-1}$ is known, just differentiate it directly.